tests/lean/run/dunfold1.lean
@@ -2,11 +2,22 @@ open tactic
 
 set_option pp.all true
 
-example (a b : nat) (p : nat → Prop) (h : p (nat.succ (nat.succ a))) : p (a + 2) :=
+def g : nat → nat := λ x, x + 5
+
+example (a b : nat) (p : nat → Prop) (h : p (g (nat.succ (nat.succ a)))) : p (g (a + 2)) :=
 by do
   t ← target,
-  new_t ← dsimplify (λ e, failed) (λ e, do new_e ← dunfold_expr e, trace e, trace "===>", trace new_e, trace "-------", return (new_e, tt)) t,
-  expected ← to_expr `(p (nat.succ (nat.succ a))),
+  new_t ← dsimplify (λ e, failed)
+     (λ e,
+        do { new_e ← unfold_projection e, return (new_e, tt) }
+        <|>
+        do {
+         guard ([`add, `nat.add, `one, `zero, `bit0, `bit1]^.any e^.is_app_of),
+         new_e ← dunfold_expr e, trace e,
+         trace "===>", trace new_e, trace "-------",
+         return (new_e, tt) })
+     t,
+  expected ← to_expr `(p (g (nat.succ (nat.succ a)))),
   guard (new_t = expected),
   trace new_t,
   assumption
